cbvlcm: Closures: stuck on translatesC_boundP proof

hol_cbvlcm2/ClosuresScript.sml
@@ -16,7 +16,7 @@ val _ = new_theory "Closures";
 Datatype:
   Clo = closC Pro (Clo list)
 End
-
+val _ = export_rewrites ["Clo_size_def"]
 (* With closures we can refine the naive stack machine
    so that no substitution operation is needed.
 *)
@@ -69,15 +69,6 @@ Theorem boundP_substP:
 Proof
   Induct_on `boundP` >> rw[] >>
   rw[Once substP]
-QED
-
-Theorem Forall_MEM:
-  ∀x H P. Forall P H ∧ MEM x H ⇒ P x
-Proof
-  Induct_on `H` >> rw[]
-  >- fs[Once Forall_cases]
-  >> qpat_x_assum `Forall P (h::H)` mp_tac >>
-  rw[Once Forall_cases]
 QED
 
 (* Fact 29.4 *)
@@ -176,15 +167,16 @@ Proof
   fs[ADD1]
 QED
 
-(*
 Definition deltaC:
   deltaC k (e: Clo) =
     case e of
       closC C E => substPl C k (MAP (deltaC 1) E)
 Termination
-
+  WF_REL_TAC `measure (λ(a, b). Clo_size b)` >> rw[] >>
+  Induct_on `E` >> rw[]
+  >- rw[]
+  >> first_x_assum drule >> rw[]
 End
-*)
 
 (*
 Definition deltaC:
@@ -195,21 +187,137 @@ End
 *)
 
 (*
-
 Notation "P / E" := (closC P E).
 
 Fixpoint δC k (e:Clo) :=
   let (C,E):=e in
   substPl C k (map (δC 1) E).
+*)
 
-Reserved Notation "P <C k" (at level 70).
+(* Reserved Notation "P <C k" (at level 70). *)
+Inductive boundC:
+  ∀k P E. boundP P (k+LENGTH E) ∧ (∀e. MEM e E ⇒ boundC e 1) ⇒ boundC (closC P E) k
+End
 
-Inductive boundC : Clo -> nat -> Prop :=
-  boundC_C k P E : P <P k+length E -> (forall e, e ∈ E -> e <C 1) -> P/E <C k
-where "e <C k" := (boundC e k).
-Notation "'(<C' k ')'" := (fun P => P <C k) (at level 0, format "'(<C' k ')'").
+Theorem translateC_boundP_1:
+  ∀e. boundC e 1 ⇒ boundP (deltaC 1 e) 1
+Proof
+  Induct >> rw[] >>
+  rw[Once deltaC] >>
+  irule substP_boundP >> rw[]
+  >- (fs[Once boundC_cases] >>
+      `∀y. MEM y (MAP (λa. deltaC 1 a) l) ⇒ (λx. boundP x 1) y`
+        suffices_by rw[Forall_forall] >> rw[] >>
+      `∃z. y = (λa. deltaC 1 a) z ∧ MEM z l`
+        by metis_tac[MEM_MAP] >>
+      first_x_assum drule >> rw[] >> )
+  >> fs[Once boundC_cases]
 
-Hint Constructors boundC.
+  fs[Once boundC_cases] >> rw[] >>
+  pop_assum mp_tac >> pop_assum mp_tac >>
+  Induct_on `boundP` >> rw[]
+  >- rw[Once deltaC, Once substPl, Once boundP_cases]
+  >- (first_x_assum drule >> rw[] >>
+      fs[Once deltaC] >> rw[Once substPl]
+      >- rw[Once boundP_cases]
+      >> fs[NOT_GREATER] >>
+      Cases_on `nth_error (n − 1) (MAP (λa. deltaC 1 a) E)` >> rw[]
+      >- (drule nth_error_NONE_lt >> rw[])
+      >> rw[Once boundP_cases] >>
+      drule nth_error_SOME_in_H >> rw[] >>
+      fs[MEM_MAP] >> rw[] >>
+
+    rw[Once deltaC, Once substPl, Once boundP_cases])
+
+  Induct >> rw[] >> pop_assum mp_tac >>
+  MAP_EVERY qid_spec_tac [`l`, `P`] >>
+  Induct_on `l` >> rw[]
+  >- (rw[Once deltaC, substPl_nil] >> fs[Once boundC_cases])
+  >> fs[Once boundC_cases] >> rw[Once deltaC] >>
+  rw[Once deltaC] >> Cases_on `h` >> rw[] >>
+
+  pop_assum mp_tac >>
+
+  rw[Once deltaC] >>
+
+  Induct >> rw[] >>
+  pop_assum mp_tac >>
+  MAP_EVERY qid_spec_tac [`l`, `P`] >>
+  Induct_on `l` >> rw[]
+  >- (rw[Once deltaC, substPl_nil] >> fs[Once boundC_cases])
+  >> rw[Once deltaC] >>
+  irule substP_boundP >> rw[]
+  >- (fs[Once boundC_cases] >>
+      `∀y. MEM y (MAP (λa. deltaC 1 a) l) ⇒ (λx. boundP x 1) y`
+        suffices_by rw[Forall_forall] >> rw[] >>
+      `∃z. y = (λa. deltaC 1 a) z ∧ MEM z l`
+        by metis_tac[MEM_MAP] >>
+      first_x_assum drule >> rw[] >>)
+  >> fs[Once boundC_cases]
+
+
+
+QED
+
+Theorem translateC_boundP:
+  ∀e k. boundC e k ⇒ boundP (deltaC k e) k
+Proof
+  Induct_on `e`
+  Cases_on `k` >> rw[]
+  >- (fs[Once boundC_cases] >> rw[Once deltaC] >>
+
+      )
+  >>
+  Induct >> rw[] >>
+  fs[Once boundC_cases] >>
+  rw[Once deltaC] >>
+  irule substP_boundP >> rw[] >>
+  `∀y. MEM y (MAP (λa. deltaC 1 a) l) ⇒ (λx. boundP x 1) y`
+    suffices_by rw[Forall_forall] >> rw[] >>
+  `∃z. y = (λa. deltaC 1 a) z ∧ MEM z l`
+    by metis_tac[MEM_MAP] >> rw[] >>
+  first_x_assum drule >> rw[] >>
+  fs[Once boundC_cases] >> rw[] >>
+  rw[Once deltaC] >>
+  rw[Once substPl] >> Cases_on `P'` >> rw[]
+  >- rw[Once boundP_cases]
+  >- (rw[Once boundP_cases] >> )
+
+  rw[Once deltaC] >> Cases_on `z` >> rw[] >>
+  first_assum drule >>
+  `boundP `
+  simp[Once boundC_cases]
+  strip_tac >>
+
+first_x_assum drule >> rw[] >>
+  boundP_substP
+  pop_assum mp_tac >> rw[Once boundC_cases] >>
+
+  rw[Once deltaC] >> Cases_on `z` >> rw[] >>
+
+
+
+
+
+  rw[] >> first_x_assum drule >> rw[] >>
+  rw[Once deltaC] >> Cases_on `z` >> rw[] >>
+  rw[Once boundP_cases]
+  `Forall (λx. boundP x 1) (MAP (λa. deltaC 1 a) l)`
+    by (Induct_on `l` >> rw[]
+        >- rw[Once Forall_cases]
+        >> )
+  rw[Once substPl] >>
+  fs[Once boundC_cases] >>
+  drule boundP_substP >> rw[] >>
+
+  rw[Once boundP_cases]
+
+  LENGTH_MAP
+  Forall_forall
+  MEM_MAP
+QED
+
+(*
 
 Lemma translateC_boundP e k:
   e <C k -> δC k e <P k.
